SciLean/Modules/SolversAndOptimizers/NewtonSolverTest.lean
@@ -5,7 +5,26 @@ open SciLean
 variable
   {R} [RealScalar R]
 
--- approximate sqrt function using newton solver
+set_default_scalar R
+
+
+
+-- direct use of newton solver
+----------------------------------------------------------------------------------------------------
+
+def mySqrt' (y : R) : R :=
+  let f := fun x : R => x^2 - y
+  let iJ := (fun x y => y/(∂! (x':=x), f x'))
+  newtonSolver {relTol := (1e-6 : R), absTol := 1e-9} f iJ y
+
+
+#eval mySqrt' 2.0
+
+
+
+-- use of newton solver through rewrites
+----------------------------------------------------------------------------------------------------
+
 approx mySqrt :=
   -- specification of sqrt function
   fun (y : R) => (fun x : R => x^2).invFun y
@@ -13,11 +32,13 @@ by
   -- rules how to construct approximation from the specification
   conv =>
     enter[2,y]
-    rw[invFun_as_newtonSolver (R:=R) 1 sorry]
+    rw[invFun_as_newtonSolver (R:=R) 1 (by fun_prop) sorry]
 
+  -- fix limit at some value `s`
   approx_limit s := sorry
 
-  fun_trans (disch:=sorry)
+  autodiff -- compute derivative
+  autodiff -- compute inverse
 
 
 -- evaluation
